Instantiate labProps line_ok_pre over a concrete AsmConfig

scripts/hol-probes/lab_props_line_ok_pre_probeScript.sml
@@ -1,0 +1,45 @@
+load "preamble";
+load "labPropsTheory";
+open bossLib;
+open HolKernel Parse;
+open preamble;
+open labPropsTheory;
+
+fun print_eval label q =
+  (print label; print "="; print_term (rconc (EVAL q)); print "\n");
+
+val cfg = ``<| ISA := RISC_V ;
+              encode := (\x. ([] : word8 list)) ;
+              big_endian := F ;
+              code_alignment := 2 ;
+              link_reg := NONE ;
+              avoid_regs := [3] ;
+              reg_count := 8 ;
+              fp_reg_count := 4 ;
+              two_reg_arith := T ;
+              valid_imm := (K (K T)) ;
+              addr_offset := (0w, 100w) ;
+              hw_offset := (0w, 100w) ;
+              byte_offset := (0w, 100w) ;
+              jump_offset := (0w, 100w) ;
+              cjump_offset := (0w, 100w) ;
+              loc_offset := (0w, 100w) |> : 8 asm_config``;
+
+val _ = print_eval "line_ok_asm_skip"
+  ``line_ok_pre ^cfg (labLang$Asm (labLang$Asmi (asm$Inst (asm$Skip : 8 asm$inst))) [] 0)``;
+val _ = print_eval "line_ok_asm_cbw"
+  ``line_ok_pre ^cfg (labLang$Asm (labLang$Cbw 1 2) [] 0)``;
+val _ = print_eval "line_ok_label"
+  ``line_ok_pre ^cfg (labLang$Label 0 1 0)``;
+val _ = print_eval "line_ok_labasm_halt"
+  ``line_ok_pre ^cfg (labLang$LabAsm labLang$Halt (0w : 8 word) [] 0)``;
+val _ = print_eval "line_ok_asm_badreg"
+  ``line_ok_pre ^cfg (labLang$Asm (labLang$Asmi (asm$Inst (asm$Const 9 (0w : 8 word)))) [] 0)``;
+val _ = print_eval "all_enc_ok_one_ok"
+  ``all_enc_ok_pre ^cfg [labLang$Section 0 [labLang$Asm (labLang$Asmi (asm$Inst (asm$Skip : 8 asm$inst))) [] 0]]``;
+val _ = print_eval "all_enc_ok_one_bad"
+  ``all_enc_ok_pre ^cfg [labLang$Section 0 [labLang$Asm (labLang$Asmi (asm$Inst (asm$Const 9 (0w : 8 word)))) [] 0]]``;
+val _ = print_eval "cbw_to_asm_store8"
+  ``cbw_to_asm (labLang$Cbw 1 2) : 8 asm$asm``;
+val _ = print_eval "cbw_to_asm_sharemem"
+  ``cbw_to_asm (labLang$ShareMem asm$Load 4 (asm$Addr 5 (0w : 8 word))) : 8 asm$asm``;
